FreydSSA/Terminator/Extrinsic/Subst.lean
@@ -6,50 +6,47 @@ import FreydSSA.Term.Extrinsic.Subst
 
 variable {φ ν α} [Φ : InstSet φ (Ty α)] [Φc : CohInstSet φ (Ty α)]
 
-def InstSet.USubst.src {σ : ν → UTm φ ν} {Γ Δ : Ctx ν (Ty α)}  (_ : Φ.USubst σ Γ Δ)
+def Ctx.Subst.src {σ : ν → UTm φ ν} {Γ Δ : Ctx ν (Ty α)}  (_ : Subst σ Γ Δ)
   : Ctx ν (Ty α) := Γ
 
-def InstSet.USubst.trg {σ : ν → UTm φ ν} {Γ Δ : Ctx ν (Ty α)}  (_ : Φ.USubst σ Γ Δ)
+def Ctx.Subst.trg {σ : ν → UTm φ ν} {Γ Δ : Ctx ν (Ty α)}  (_ : Subst σ Γ Δ)
   : Ctx ν (Ty α) := Δ
 
-inductive InstSet.USubstL (σ : ν → UTm φ ν)
+inductive LCtx.Subst (σ : ν → UTm φ ν)
   : LCtx ν κ (Ty α) → LCtx ν κ (Ty α) → Type _
-  | nil : USubstL σ [] []
-  | cons (n A) : USubst σ Γ Δ → USubstL σ L K → USubstL σ (⟨n, A, Γ⟩ :: L) (⟨n, A, Δ⟩ :: K)
-  | skip : L.Fresh ℓ.name → USubstL σ L K → USubstL σ L (ℓ :: K)
+  | nil : Subst σ [] []
+  | cons (n A) : Γ.Subst σ Δ → Subst σ L K → Subst σ (⟨n, A, Γ⟩ :: L) (⟨n, A, Δ⟩ :: K)
+  | skip : L.Fresh ℓ.name → Subst σ L K → Subst σ L (ℓ :: K)
 
-def InstSet.USubstL.ofEmpty
+def LCtx.Subst.ofEmpty
   (σ : ν → UTm φ ν)
   {L : LCtx ν κ (Ty α)}
-  : (LCtx.Wk [] L) → USubstL σ [] L
+  : (LCtx.Wk [] L) → Subst σ [] L
   | LCtx.Wk.nil => nil
   | LCtx.Wk.skip hℓ w => skip hℓ (ofEmpty σ w)
 
-def InstSet.USubstL.ofVar {σ : ν → UTm φ ν}
-  {Γ Δ : Ctx ν (Ty α)}
-  {n A}
-  (hσ : USubst σ Γ Δ)
-  : {L : LCtx ν κ (Ty α)} → LCtx.Wk [⟨n, A, Δ⟩] L → USubstL σ [⟨n, A, Γ⟩] L
+def LCtx.Subst.ofVar {σ : ν → UTm φ ν}
+  {Γ Δ : Ctx ν (Ty α)} {n A} (hσ : Γ.Subst σ Δ)
+  : {L : LCtx ν κ (Ty α)} → LCtx.Wk [⟨n, A, Δ⟩] L → Subst σ [⟨n, A, Γ⟩] L
   | ⟨_, _, _Δ'⟩::_, LCtx.Wk.cons ⟨rfl, rfl, wΔ⟩ w => cons _ _ (hσ.wk_exit wΔ) (ofEmpty σ w)
   | _::_, LCtx.Wk.skip hℓ w => skip (LCtx.Fresh.of_not_mem hℓ.not_mem) (ofVar hσ w)
 
-theorem LCtx.Fresh.subst {L K : LCtx ν κ (Ty α)}
-  : Φ.USubstL σ L K → K.Fresh ℓ → L.Fresh ℓ
-  | InstSet.USubstL.nil, nil => nil
-  | InstSet.USubstL.cons _ _ _ hσL, cons h f => cons h (subst hσL f)
-  | InstSet.USubstL.skip _ hσL, cons h' f => subst hσL f
+theorem LCtx.Fresh.subst {σ : ν → UTm φ ν} {L K : LCtx ν κ (Ty α)}
+  : Subst σ L K → K.Fresh ℓ → L.Fresh ℓ
+  | Subst.nil, nil => nil
+  | Subst.cons _ _ _ hσL, cons h f => cons h (subst hσL f)
+  | Subst.skip _ hσL, cons h' f => subst hσL f
 
-def InstSet.USubstL.wk_exit {σ : ν → UTm φ ν}
-  {L K K' : LCtx ν κ (Ty α)}
-  : USubstL σ L K → LCtx.Wk K K' → USubstL σ L K'
+def LCtx.Subst.wk_exit {σ : ν → UTm φ ν} {L K K' : LCtx ν κ (Ty α)}
+  : Subst σ L K → LCtx.Wk K K' → Subst σ L K'
   | nil, LCtx.Wk.nil => nil
   | cons n A h hσ, @LCtx.Wk.cons _ _ _ _ _ ⟨_, _, _⟩ ⟨_, _, _⟩ ⟨hn, hp, w⟩ w'
     => by cases hn; cases hp; exact cons n A (h.wk_exit w) (wk_exit hσ w')
   | skip h hσ, LCtx.Wk.cons hℓ w' => skip (hℓ.name ▸ h) (wk_exit hσ w')
   | hσ, LCtx.Wk.skip h' w => skip (h'.subst hσ) (wk_exit hσ w)
 
-theorem InstSet.USubstL.allEq {σ : ν → UTm φ ν} {L K : LCtx ν κ (Ty α)}
-  : (hσ  hσ': Φ.USubstL σ L K) → hσ = hσ'
+theorem LCtx.Subst.allEq {σ : ν → UTm φ ν} {L K : LCtx ν κ (Ty α)}
+  : (hσ hσ': Subst σ L K) → hσ = hσ'
   | nil, nil => rfl
   | cons n A h hσ, cons _ _ h' hσ' => by
     cases h.allEq h'
@@ -61,52 +58,52 @@ theorem InstSet.USubstL.allEq {σ : ν → UTm φ ν} {L K : LCtx ν κ (Ty α)}
   | cons _ _ _ _, skip h _ => (h.head rfl).elim
   | skip h _, cons _ _ _ _ => (h.head rfl).elim
 
-inductive InstSet.USubstLP [Φ : InstSet φ (Ty α)] (σ : ν → UTm φ ν)
+inductive LCtx.PSubst [Φ : InstSet φ (Ty α)] (σ : ν → UTm φ ν)
   : LCtx ν κ (Ty α) → LCtx ν κ (Ty α) → Type _
-  | nil : USubstLP σ [] []
-  | cons (n A) : USubst σ Γ Δ → USubstLP σ L K → USubstLP σ (⟨n, A, Γ⟩ :: L) (⟨n, A, Δ⟩ :: K)
+  | nil : PSubst σ [] []
+  | cons (n A) : Γ.Subst σ Δ → PSubst σ L K → PSubst σ (⟨n, A, Γ⟩ :: L) (⟨n, A, Δ⟩ :: K)
 
-theorem InstSet.USubstLP.allEq {σ : ν → UTm φ ν} {L K : LCtx ν κ (Ty α)}
-  : (hσ  hσ': Φ.USubstLP σ L K) → hσ = hσ'
+theorem LCtx.PSubst.allEq {σ : ν → UTm φ ν} {L K : LCtx ν κ (Ty α)}
+  : (hσ  hσ': PSubst σ L K) → hσ = hσ'
   | nil, nil => rfl
   | cons n A h hσ, cons _ _ h' hσ' => by
     cases h.allEq h'
     cases hσ.allEq hσ'
     rfl
 
-def InstSet.USubstLP.pwk_exit {σ : ν → UTm φ ν} {L K K' : LCtx ν κ (Ty α)}
-  : Φ.USubstLP σ L K → LCtx.PWk K K' → Φ.USubstLP σ L K'
-  | nil, LCtx.PWk.nil => InstSet.USubstLP.nil
+def LCtx.PSubst.pwk_exit {σ : ν → UTm φ ν} {L K K' : LCtx ν κ (Ty α)}
+  : PSubst σ L K → LCtx.PWk K K' → PSubst σ L K'
+  | nil, LCtx.PWk.nil => nil
   | cons n A h hσ, @LCtx.PWk.cons _ _ _ _ _ ⟨_, _, _⟩ ⟨_, _, _⟩ ⟨hn, hp, w'⟩ w =>
     by cases hn; cases hp; exact cons n A (h.wk_exit w') (hσ.pwk_exit w)
 
-def InstSet.USubstLP.toUSubstL {σ : ν → UTm φ ν} {L K : LCtx ν κ (Ty α)}
-  : Φ.USubstLP σ L K → Φ.USubstL σ L K
-  | InstSet.USubstLP.nil => InstSet.USubstL.nil
-  | InstSet.USubstLP.cons n A h hσ => InstSet.USubstL.cons n A h (toUSubstL hσ)
+def LCtx.PSubst.toSubst {σ : ν → UTm φ ν} {L K : LCtx ν κ (Ty α)}
+  : PSubst σ L K → Subst σ L K
+  | nil => Subst.nil
+  | cons n A h hσ => Subst.cons n A h (toSubst hσ)
 
-theorem LCtx.Fresh.substP {L K : LCtx ν κ (Ty α)}
-  : Φ.USubstLP σ L K → K.Fresh ℓ → L.Fresh ℓ
-  | InstSet.USubstLP.nil, nil => nil
-  | InstSet.USubstLP.cons _ _ _ hσL, cons h f => cons h (substP hσL f)
+theorem LCtx.Fresh.psubst {σ : ν → UTm φ ν} {L K : LCtx ν κ (Ty α)}
+  : PSubst σ L K → K.Fresh ℓ → L.Fresh ℓ
+  | PSubst.nil, nil => nil
+  | PSubst.cons _ _ _ hσL, cons h f => cons h (psubst hσL f)
 
-theorem LCtx.Fresh.rsubstP {L K : LCtx ν κ (Ty α)}
-  : Φ.USubstLP σ L K → L.Fresh ℓ → K.Fresh ℓ
-  | InstSet.USubstLP.nil, nil => nil
-  | InstSet.USubstLP.cons _ _ _ hσL, cons h f => cons h (rsubstP hσL f)
+theorem LCtx.Fresh.psubst_r {σ : ν → UTm φ ν} {L K : LCtx ν κ (Ty α)}
+  : PSubst σ L K → L.Fresh ℓ → K.Fresh ℓ
+  | PSubst.nil, nil => nil
+  | PSubst.cons _ _ _ hσL, cons h f => cons h (psubst_r hσL f)
 
-def InstSet.USubstLP.antiSJoin {σ : ν → UTm φ ν}
+def LCtx.PSubst.antiSJoin {σ : ν → UTm φ ν}
   {Γ : Ctx ν (Ty α)} {L K M L' K' : LCtx ν κ (Ty α)}
-  : Φ.USubstLP σ L' L → Φ.USubstLP σ K' K → L.SJoin K M
+  : PSubst σ L' L → PSubst σ K' K → L.SJoin K M
     → Γ.LEq L' → Γ.LEq K'
-    → (M' : LCtx ν κ (Ty α)) ×' L'.SJoin K' M' × Φ.USubstLP σ M' M
+    → (M' : LCtx ν κ (Ty α)) ×' L'.SJoin K' M' × PSubst σ M' M
   | nil, nil, LCtx.SJoin.nil => λ_ _ => ⟨[], LCtx.SJoin.nil, nil⟩
   | cons n A hσ hσL, hσK, LCtx.SJoin.left h j => λhL hK =>
     let j' := antiSJoin hσL hσK j hL.tail hK;
-    ⟨_, j'.2.1.left (h.substP hσK), j'.2.2.cons _ _ hσ⟩
+    ⟨_, j'.2.1.left (h.psubst hσK), j'.2.2.cons _ _ hσ⟩
   | hσL, cons n A hσ' hσK, LCtx.SJoin.right h j => λhL hK =>
     let j' := antiSJoin hσL hσK j hL hK.tail;
-    ⟨_, j'.2.1.right (h.substP hσL), j'.2.2.cons _ _ hσ'⟩
+    ⟨_, j'.2.1.right (h.psubst hσL), j'.2.2.cons _ _ hσ'⟩
   | cons n A _ hσL, cons _ _ hσ' hσK, LCtx.SJoin.both _ j => λhL hK  =>
     let j' := antiSJoin hσL hσK j hL.tail hK.tail;
     have hΓ := hL.head.symm.trans hK.head;
@@ -114,50 +111,50 @@ def InstSet.USubstLP.antiSJoin {σ : ν → UTm φ ν}
 
 def UTerminator.WfM.subst {t : UTerminator φ ν κ}
   {σ : ν → UTm φ ν}
-  (hσ : Φ.USubst σ Γ Δ)
-  : t.WfM Δ K → (L : LCtx ν κ (Ty α)) ×' (t.rewrite σ).WfM Γ L × Φ.USubstLP σ L K
-  | br ℓ de => ⟨_, br ℓ (de.subst hσ), InstSet.USubstLP.nil.cons _ _ hσ⟩
+  (hσ : Γ.Subst σ Δ)
+  : t.WfM Δ K → (L : LCtx ν κ (Ty α)) ×' (t.rewrite σ).WfM Γ L × L.PSubst σ K
+  | br ℓ de => ⟨_, br ℓ (de.subst hσ), LCtx.PSubst.nil.cons _ _ hσ⟩
   | ite dc dt df j =>
     let ⟨_, dt', hLt⟩ := subst hσ dt;
     let ⟨_, df', hLf⟩ := subst hσ df;
     let ⟨L, j', hL⟩ := hLt.antiSJoin hLf j dt'.lEq df'.lEq;
     ⟨L, ite (dc.subst hσ) dt' df' j', hL⟩
 
-structure InstSet.USubstL' [Φ : InstSet φ (Ty α)]
+structure LCtx.Subst' [Φ : InstSet φ (Ty α)]
   (σ : ν → UTm φ ν) (L K : LCtx ν κ (Ty α)) where
   mapped : LCtx ν κ (Ty α)
-  uSubstLP : Φ.USubstLP σ L mapped
+  pSubst : PSubst σ L mapped
   wk : mapped.EWk K
 
-def InstSet.USubstL.factor [Φ : InstSet φ (Ty α)]
+def LCtx.Subst.factor [Φ : InstSet φ (Ty α)]
   {σ : ν → UTm φ ν} {L K : LCtx ν κ (Ty α)}
-  : Φ.USubstL σ L K → Φ.USubstL' σ L K
-  | nil => ⟨[], USubstLP.nil, LCtx.EWk.nil⟩
+  : Subst σ L K → Subst' σ L K
+  | nil => ⟨[], PSubst.nil, LCtx.EWk.nil⟩
   | cons n A hσ' hσL =>
     let hσL' := factor hσL;
-    ⟨_, hσL'.uSubstLP.cons n A hσ', hσL'.wk.cons _⟩
+    ⟨_, hσL'.pSubst.cons n A hσ', hσL'.wk.cons _⟩
   | skip h hσL =>
     let hσL' := factor hσL;
-    ⟨_, hσL'.uSubstLP, hσL'.wk.skip (h.rsubstP hσL'.uSubstLP)⟩
+    ⟨_, hσL'.pSubst, hσL'.wk.skip (h.psubst_r hσL'.pSubst)⟩
 
-def InstSet.USubstL'.toUSubstL [Φ : InstSet φ (Ty α)]
+def LCtx.Subst'.toSubst [Φ : InstSet φ (Ty α)]
   {σ : ν → UTm φ ν} {L K : LCtx ν κ (Ty α)}
-  (hσ : Φ.USubstL' σ L K) : Φ.USubstL σ L K
-  := hσ.uSubstLP.toUSubstL.wk_exit hσ.wk.toWk
+  (hσ : Subst' σ L K) : Subst σ L K
+  := hσ.pSubst.toSubst.wk_exit hσ.wk.toWk
 
 --TODO: USubstL'.allEq...
 
 def UTerminator.Wf'.subst
   {t : UTerminator φ ν κ}
-  (hσ : Φ.USubst σ Γ Δ)
-  (dt : t.Wf' Δ K) : (L : LCtx ν κ (Ty α)) ×' (t.rewrite σ).Wf' Γ L × Φ.USubstL' σ L K :=
+  (hσ : Γ.Subst σ Δ)
+  (dt : t.Wf' Δ K) : (L : LCtx ν κ (Ty α)) ×' (t.rewrite σ).Wf' Γ L × L.Subst' σ K :=
   let dt' := dt.wfM.subst hσ;
   let wk' := dt.wk.factor
   ⟨_, dt'.2.1.toWf', ⟨_, dt'.2.2.pwk_exit wk'.pWk, wk'.eWk⟩⟩
 
 def UTerminator.Wf.subst
   {t : UTerminator φ ν κ}
-  (hσ : Φ.USubst σ Γ Δ)
-  (dt : t.Wf Δ K) : (L : LCtx ν κ (Ty α)) ×' (t.rewrite σ).Wf Γ L × Φ.USubstL σ L K :=
+  (hσ : Γ.Subst σ Δ)
+  (dt : t.Wf Δ K) : (L : LCtx ν κ (Ty α)) ×' (t.rewrite σ).Wf Γ L × L.Subst σ K :=
   let dt' := dt.factor.subst hσ;
-  ⟨dt'.1, dt'.2.1.toWf, dt'.2.2.toUSubstL⟩
+  ⟨dt'.1, dt'.2.1.toWf, dt'.2.2.toSubst⟩
